RefinementTypeProp.v
@@ -303,6 +303,9 @@ Proof.
   my_set_solver.
 Qed.
 
+Lemma open_rec_lc_rty: ∀ (u : value) τ (k : nat), lc_rty τ -> {k ~r> u} τ = τ.
+Admitted.
+
 (* Lemma closed_rty_td_congr d ρ a : *)
 (*   closed_rty d ρ -> *)
 (*   pure_rty ρ -> *)
